wip

cedar-lean/Cedar/Thm/EntitySlice.lean
@@ -580,7 +580,25 @@ theorem no_euids_in_reqty_means_no_euids_in_context : ∀ env request entities l
     apply no_euids
 
 
+def evalsToRecord (e : Expr) : Prop :=
+  ∀ entities request env (c₁ c₂ : Capabilities) rty rv,
+    typeOf e c₁ env (.finite 1 == Level.infinite) = .ok (.record rty, c₂) →
+    CapabilitiesInvariant c₁ request entities →
+    RequestAndEntitiesMatchEnvironmentLeveled env request entities (.finite 1) →
+    NoEuidsInEnv env →
+    evaluate e request entities = .ok (Value.record rv) →
+    NoEuidValues (.record rv)
 
+theorem evals_to_record (e : Expr) entities request env c₁ c₂ rty rv
+  (well_typed : typeOf e c₁ env (.finite 1 == Level.infinite) = .ok (.record rty, c₂))
+  (non_zero : l ≠ Level.zero)
+  (caps_inv : CapabilitiesInvariant c₁ request entities)
+  (req_well_typed : RequestAndEntitiesMatchEnvironmentLeveled env request entities (.finite 1))
+  (no_euids : NoEuidsInEnv env)
+  (is_record : evaluate e request entities = .ok (Value.record rv)) :
+  NoEuidValues (.record rv)
+  := by
+  sorry
 
 def evalsToEuid (e : Expr) : Prop :=
   ∀ entities request env (c₁ c₂ : Capabilities) ety l euid,
@@ -590,13 +608,13 @@ def evalsToEuid (e : Expr) : Prop :=
     RequestAndEntitiesMatchEnvironmentLeveled env request entities (.finite 1) →
     NoEuidsInEnv env →
     evaluate e request entities = .ok (Value.prim (.entityUID euid)) →
-    (euid ∈ [request.principal, request.action, request.resource])
+    (euid ∈ [request.principal, request.action, request.resource]) ∧ l = Level.finite 1
 
 theorem evals_to_euid_lit (p : Prim) entities request env c₁ c₂ ety l euid
   (well_typed : typeOf (.lit p) c₁ env (.finite 1 == Level.infinite) = .ok (.entity ety l, c₂))
   (non_zero : l ≠ Level.zero)
   (is_euid : evaluate (.lit p) request entities = .ok (Value.prim (.entityUID euid))) :
-  (euid ∈ [request.principal, request.action, request.resource])
+  (euid ∈ [request.principal, request.action, request.resource]) ∧ l = Level.finite 1
   := by
   cases p <;> simp [evaluate] at is_euid
   case _ =>
@@ -618,16 +636,22 @@ theorem evals_to_euid_lit (p : Prim) entities request env c₁ c₂ ety l euid
 
 theorem evals_to_euid_var (v : Var) entities request env c₁ c₂ ety l euid
   (well_typed : typeOf (.var v) c₁ env (.finite 1 == Level.infinite) = .ok (.entity ety l, c₂))
+  (req_well_typed : RequestAndEntitiesMatchEnvironmentLeveled env request entities (.finite 1))
   (is_euid : evaluate (.var v) request entities = .ok (Value.prim (.entityUID euid))) :
-  (euid ∈ [request.principal, request.action, request.resource])
+  (euid ∈ [request.principal, request.action, request.resource]) ∧ l = .finite 1
   := by
-  cases v
-    <;>
-    simp [evaluate] at is_euid
-    <;> (
-    subst is_euid
-    simp
-    )
+  cases v <;>
+  simp [evaluate] at is_euid <;> constructor
+  <;> try simp [is_euid]
+  all_goals {
+    simp [RequestAndEntitiesMatchEnvironmentLeveled] at req_well_typed
+    have h := req_well_typed.left
+    simp [InstanceOfRequestTypeLevel] at h
+    simp [typeOf,typeOfVar, ok] at well_typed
+    have h₂ := well_typed.left.right
+    simp [h] at h₂
+    simp [h₂]
+  }
 
 theorem levels_nonzero {l l' : Level}
   (l_not_zero : l ≠ .finite 0)
@@ -647,6 +671,30 @@ theorem levels_nonzero {l l' : Level}
     omega
 
 
+theorem le_one_and_zero (l₁ l₂ : Level)
+  (h₁ : l₁ ≠ .finite 0)
+  (h₂ : l₂ = .finite 1)
+  (h₃ : l₁ ≤ l₂) :
+  l₁ = .finite 1 := by
+  cases l₁ <;> cases l₂
+  case _ =>
+    cases h₂
+  case _ =>
+    cases h₃
+  case _ =>
+    cases h₂
+  case _ n₁ n₂ =>
+    simp [Level.finite] at h₂
+    subst h₂
+    simp [LE.le] at h₃
+    cases h₃
+    case _ h =>
+      subst h
+      simp [Level.finite]
+    case _ h =>
+      cases h
+      simp [Level.finite] at h₁
+      omega
 
 theorem evals_to_euid_ite (cond cons alt : Expr) entities request env c₁ c₂ ety l euid
   (well_typed : typeOf (.ite cond cons alt)  c₁ env (.finite 1 == Level.infinite) = .ok (.entity ety l, c₂))
@@ -657,7 +705,7 @@ theorem evals_to_euid_ite (cond cons alt : Expr) entities request env c₁ c₂ 
   (is_euid : evaluate (.ite cond cons alt) request entities = .ok (Value.prim (.entityUID euid)))
   (ih₁ : evalsToEuid cons)
   (ih₂ : evalsToEuid alt) :
-  (euid ∈ [request.principal, request.action, request.resource])
+  (euid ∈ [request.principal, request.action, request.resource]) ∧ l = .finite 1
   := by
   have ⟨bty, c₁', ty₂, c₂', ty₃, c₃, hinv₁, hinv⟩ := type_of_ite_inversion well_typed
   have ⟨gcaps_inv, v_cond, sound₁, sound₂⟩ : GuardedCapabilitiesInvariant cond c₁' request entities ∧ ∃ v, EvaluatesToLeveled cond request entities v  ∧ InstanceOfType v (.bool bty) := by
@@ -714,19 +762,24 @@ theorem evals_to_euid_ite (cond cons alt : Expr) entities request env c₁ c₂ 
         simp [hinv]
       have typed_as_entity := hinv.left
       rw [step₁] at typed_as_entity
-      apply ih₁
-      apply typed_as_entity
+      simp only [evalsToEuid] at ih₁
       have step₂ : l ≤ l' := by
         apply lub_to_entity_level_bound ty₃ ety l' l
         rw [lub_comm]
         rw [← step₁]
         simp [hinv]
-      apply levels_nonzero
-      apply non_zero
-      apply step₂
-      apply capability_union_invariant
-      assumption
-      apply gcaps_inv
+      have ⟨euid_is_good, lub_level_one⟩ : euid ∈ [request.principal, request.action, request.resource] ∧ (l' = .finite 1) := by
+        apply ih₁
+        apply typed_as_entity
+        apply levels_nonzero
+        apply non_zero
+        apply step₂
+        apply capability_union_invariant
+        assumption
+        apply gcaps_inv
+        repeat assumption
+      simp [euid_is_good]
+      apply le_one_and_zero
       repeat assumption
     case false =>
       rcases sound₁ with evals | evals | evals
@@ -742,22 +795,195 @@ theorem evals_to_euid_ite (cond cons alt : Expr) entities request env c₁ c₂ 
         apply lub_to_entity_level_bound ty₂ ety l' l
         rw [← step₁]
         simp [hinv]
+      have ⟨euid_is_good, lub_is_one⟩ := euid ∈ [request.principal, request]
       apply levels_nonzero
       apply non_zero
       repeat assumption
 
-theorem evals_to_euid_and (lhs rhs : Expr) entities request env c₁ c₂ ety l euid
-  (well_typed : typeOf (.and lhs rhs) c₁ env (.finite 1 == Level.infinite) = .ok (.entity ety l, c₂))
+theorem evals_to_euid_and (lhs rhs : Expr) entities request euid
+  (is_euid : evaluate (.and lhs rhs) request entities = .ok (Value.prim (.entityUID euid))) :
+  (euid ∈ [request.principal, request.action, request.resource])
+  := by
+  cases eval_lhs : (evaluate lhs request entities) <;> cases eval_rhs : (evaluate rhs request entities)
+    <;> simp [evaluate, eval_rhs, eval_lhs, Result.as, Coe.coe, Value.asBool] at is_euid
+    <;> rename Value => v
+  case _ =>
+    cases v
+    case _  p =>
+      cases p
+      case bool b =>
+        cases b <;> simp at is_euid
+      all_goals { simp at is_euid }
+    all_goals { simp at is_euid }
+  case _ v' =>
+    cases v'
+    case prim p =>
+      cases p
+      case bool b =>
+        cases b <;> simp at is_euid
+        cases v
+        case prim p =>
+          cases p
+          case bool b =>
+            cases b <;> simp [pure, Except.pure] at is_euid
+          all_goals { simp at is_euid }
+        all_goals { simp at is_euid }
+      all_goals { simp at is_euid }
+    all_goals { simp at is_euid }
+
+
+theorem evals_to_euid_or (lhs rhs : Expr) entities request euid
+  (is_euid : evaluate (.or lhs rhs) request entities = .ok (Value.prim (.entityUID euid))) :
+  (euid ∈ [request.principal, request.action, request.resource])
+  := by
+  cases eval_lhs : (evaluate lhs request entities) <;> simp [evaluate, eval_lhs, Result.as, Coe.coe, Value.asBool] at is_euid
+  rename Value => v
+  cases v <;> try simp at is_euid
+  rename Prim => p
+  cases p <;> try simp at is_euid
+  rename Bool => b
+  cases b <;> simp at is_euid
+  cases eval_rhs : (evaluate rhs request entities) <;> simp [evaluate, eval_rhs, Result.as, Coe.coe]  at is_euid
+  rename Value => v
+  cases v <;> try simp at is_euid
+  rename Prim => p
+  cases p <;> try simp at is_euid
+  rename Bool => b
+  cases b <;> simp [pure, Except.pure] at is_euid
+
+
+theorem evals_to_euid_unop (e : Expr) (o : UnaryOp) entities request euid
+  (is_euid : evaluate (.unaryApp o e) request entities = .ok (Value.prim (.entityUID euid))) :
+  (euid ∈ [request.principal, request.action, request.resource])
+  := by
+  cases eval : evaluate e request entities <;> simp [evaluate, eval, Result.as]  at is_euid
+  rename Value => v
+  cases o <;>  cases v <;> simp [apply₁] at is_euid
+  <;> rename Prim => p
+  case _ =>
+    cases p <;> simp at is_euid
+  case _ =>
+    cases p <;> simp [intOrErr] at is_euid
+    rename_i i
+    cases neg :  (i.neg?) <;> simp [neg] at is_euid
+  case _ =>
+    cases p <;> simp at is_euid
+  case _ =>
+    cases p <;> simp at is_euid
+
+theorem evals_to_euid_binop (o : BinaryOp) (lhs rhs : Expr) entities request euid
+  (is_euid : evaluate (.binaryApp o lhs rhs) request entities = .ok (Value.prim (.entityUID euid))) :
+  (euid ∈ [request.principal, request.action, request.resource])
+  := by
+  cases eval_lhs : evaluate lhs request entities <;> simp [evaluate, eval_lhs, Coe.coe] at is_euid
+  cases eval_rhs : evaluate rhs request entities <;> simp [evaluate, eval_rhs, Coe.coe] at is_euid
+  rename_i lhs rhs
+  simp [apply₂] at is_euid
+  cases o
+  case _ =>
+    cases lhs <;> cases rhs <;> simp at is_euid
+  case _ =>
+    cases lhs <;> cases rhs
+    case prim.prim =>
+      rename_i lhs rhs
+      cases lhs <;> cases rhs <;> simp at is_euid
+    case prim.set =>
+      rename_i lhs rhs
+      cases lhs <;> simp at is_euid
+      rename EntityUID => euid
+      simp [inₛ] at is_euid
+      cases find : rhs.mapOrErr Value.asEntityUID Error.typeError
+      <;> simp [find] at is_euid
+    all_goals { simp at is_euid }
+  case _ =>
+    cases lhs <;> try simp at is_euid
+    case prim p =>
+    cases p <;> try simp at is_euid
+    case int i =>
+    cases rhs  <;> try simp at is_euid
+    case prim p =>
+    cases p  <;> simp at is_euid
+  case _ =>
+    cases lhs <;> try simp at is_euid
+    case prim p =>
+    cases p <;> try simp at is_euid
+    case int i =>
+    cases rhs  <;> try simp at is_euid
+    case prim p =>
+    cases p  <;> simp at is_euid
+  case _ =>
+    cases lhs <;> try simp at is_euid
+    case prim p =>
+    cases p <;> try simp at is_euid
+    case int i =>
+    cases rhs  <;> try simp at is_euid
+    case prim p =>
+    cases p  <;> simp at is_euid
+    rename_i j
+    <;> simp [intOrErr] at is_euid
+    cases h : (i.add? j)
+    <;> simp [h]at is_euid
+  case _ =>
+    cases lhs <;> try simp at is_euid
+    case prim p =>
+    cases p <;> try simp at is_euid
+    case int i =>
+    cases rhs  <;> try simp at is_euid
+    case prim p =>
+    cases p  <;> simp at is_euid
+    rename_i j
+    <;> simp [intOrErr] at is_euid
+    cases h : (i.sub? j)
+    <;> simp [h] at is_euid
+  case _ =>
+    cases lhs <;> try simp at is_euid
+    case prim p =>
+    cases p <;> try simp at is_euid
+    case int i =>
+    cases rhs  <;> try simp at is_euid
+    case prim p =>
+    cases p  <;> simp at is_euid
+    rename_i j
+    <;> simp [intOrErr] at is_euid
+    cases h : (i.mul? j)
+    <;> simp [h] at is_euid
+  case _ =>
+    cases lhs <;> simp at is_euid
+  case _ =>
+    cases lhs <;> try simp at is_euid
+    cases rhs <;> simp at is_euid
+  case _ =>
+    cases lhs <;> try simp at is_euid
+    cases rhs <;> simp at is_euid
+
+theorem evals_to_euid_getAttr (attr : Attr) (e : Expr) entities request env c₁ c₂ ety l euid
+  (well_typed : typeOf (e.getAttr attr) c₁ env (.finite 1 == Level.infinite) = .ok (.entity ety l, c₂))
   (non_zero : l ≠ Level.zero)
   (caps_inv : CapabilitiesInvariant c₁ request entities)
   (req_well_typed : RequestAndEntitiesMatchEnvironmentLeveled env request entities (.finite 1))
   (no_euids : NoEuidsInEnv env)
-  (is_euid : evaluate (.and lhs rhs) request entities = .ok (Value.prim (.entityUID euid))) :
+  (is_euid : evaluate (e.getAttr attr) request entities = .ok (Value.prim (.entityUID euid))) :
   (euid ∈ [request.principal, request.action, request.resource])
   := by
+  have hinv := type_of_getAttr_inversion_levels well_typed
+  replace ⟨hinv₁, c₁', hinv⟩ := hinv
+  cases hinv
+  case _ hinv =>
+    replace ⟨ety', l₂, hinv₂, hinv⟩ := hinv
+    simp [typeOf, hinv₂, typeOfGetAttr] at well_typed
+    rw [if_pos] at well_typed
+    cases find_types : env.ets.attrs? ety'
+    <;> simp [find_types, err]at well_typed
 
-  sorry
 
+
+
+
+
+
+    sorry
+  case _ hinv =>
+    sorry
 
 theorem evals_to_euid (e : Expr) entities request env c₁ c₂ ety l euid
   (well_typed : typeOf e c₁ env (.finite 1 == Level.infinite) = .ok (.entity ety l, c₂))
@@ -785,15 +1011,19 @@ theorem evals_to_euid (e : Expr) entities request env c₁ c₂ ety l euid
       repeat assumption
     }
   case and lhs rhs =>
+    apply evals_to_euid_and
+    repeat assumption
+  case _ =>
+    apply evals_to_euid_or
+    repeat assumption
+  case _ =>
+    apply evals_to_euid_unop
+    repeat assumption
+  case _ =>
+    apply evals_to_euid_binop
+    repeat assumption
+  case _ =>
 
-    sorry
-  case _ =>
-    sorry
-  case _ =>
-    sorry
-  case _ =>
-    sorry
-  case _ =>
     sorry
   case _ =>
     sorry
